1) extracted new properties of the memory model. The memory_props.v should be movied to ./src/Vellvm later 2) Found a problem of malloc: malloc should ensure that all elements in an allocated aggregated object are well-aligned.
git-svn-id: https://webdav.seas.upenn.edu/svn/sol/vol@3580 eef5ea85-cc2e-0410-bd84-0fae1f012da8

src/Transforms/promotable_props.v
@@ -15,8 +15,11 @@ Require Import primitives.
 Require Import Maps.
 Require Import mem2reg.
 Require Import opsem_props.
+Require Import memory_props.
 
 Module Promotability.
+
+Export MemProps.
 
 Definition DGVMap := @Opsem.GVsMap DGVs.
 
@@ -46,39 +49,6 @@ succs = successors f /\
 preds = make_predecessors succs /\
 newids = fst (gen_fresh_ids rd (getFdefLocs f)).
 
-(* wf_global and wf_globals are copied from sb_ds_gv_inject.v 
-   We should move the invariant to memory model. *)
-Fixpoint wf_global (maxb:Values.block) (gv:GenericValue) 
-  : Prop :=
-match gv with
-| nil => True
-| (Vptr b _,_)::gv' => b <= maxb /\ wf_global maxb gv'
-| _::gv' => wf_global maxb gv'
-end.
-
-Fixpoint wf_global_list maxb (gl:GVMap) : Prop :=
-match gl with
-| nil => True
-| (_,gv)::gl' => wf_global maxb gv /\ wf_global_list maxb gl'
-end.
-
-Definition wf_globals maxb (gl:GVMap) : Prop :=
-0 <= maxb /\ wf_global_list maxb gl.
-
-Fixpoint no_alias_with_blk (gvs:GenericValue) (blk:Values.block) : Prop :=
-match gvs with
-| nil => True
-| (Vptr b _,_)::gvs' => b <> blk /\ no_alias_with_blk gvs' blk
-| _::gvs' => no_alias_with_blk gvs' blk
-end.
-
-Fixpoint no_alias (gvs1 gvs2:GenericValue) : Prop :=
-match gvs2 with
-| nil => True
-| (Vptr b _,_)::gvs2' => no_alias_with_blk gvs1 b /\ no_alias gvs1 gvs2'
-| _::gvs2' => no_alias gvs1 gvs2'
-end.
-
 Definition wf_non_alloca_GVs (pinfo:PhiInfo) (id1:id) (gvs1 gvsa:GenericValue) 
   : Prop :=
 (if (id_dec id1 (PI_id pinfo)) then True else no_alias gvs1 gvsa).
@@ -103,17 +73,6 @@ forall gvsa
    (*Hin0: In id0 ids0*) 
    (Hlk0: lookupAL _ lc id0 = Some gvs0),
    wf_non_alloca_GVs pinfo id0 gvs0 gvsa).
-
-Fixpoint valid_ptrs (bound:Values.block) (gvs:GenericValue): Prop :=
-match gvs with
-| nil => True
-| (Vptr blk _,_)::gvs' => blk < bound /\ valid_ptrs bound gvs'
-| _::gvs' => valid_ptrs bound gvs'
-end.
-
-Definition wf_lc M lc : Prop :=
-forall id0 gvs, 
-  lookupAL _ lc id0 = Some gvs -> valid_ptrs (Mem.nextblock M) gvs.
 
 Definition inscope_of_pc f b cs tmn : option (list id) :=
 match cs with
@@ -166,14 +125,6 @@ match ecs with
     wf_ECStack maxb pinfo TD M ecs' /\
     wf_ECStack_head_tail maxb pinfo TD M (Opsem.Locals ec) ecs'
 end.
-
-Definition wf_Mem maxb (td:targetdata) (M:mem) : Prop :=
-(forall gptr ty al gvs, 
-  mload td M gptr ty al = Some gvs -> valid_ptrs (Mem.nextblock M) gvs) /\
-maxb < Mem.nextblock M.
-
-Definition wf_als maxb M (als: list Values.block) : Prop :=
-NoDup als /\ (forall al, In al als -> maxb < al < Mem.nextblock M).
 
 Definition wf_State (maxb:Values.block) (pinfo:PhiInfo) (cfg:OpsemAux.Config) 
   (S:Opsem.State) : Prop :=
@@ -357,9 +308,16 @@ Proof.
 Qed.
 
 (* We need a generic proof for this one and the one for atom *)
-Lemma NoDup_disjoint : forall (l1 l2 : list Z) (i0 : Z),
+Lemma NoDup_disjoint : forall (l2 l1 : list Z) (i0 : Z),
   NoDup (l1 ++ l2) -> In i0 l2 -> ~ In i0 l1.
-Admitted.
+Proof.
+  induction l1; simpl; intros; auto.
+    inv H.
+    intro J. 
+    destruct J as [J | J]; subst.
+      apply H3. apply in_or_app. auto.
+      eapply IHl1 in H4; eauto.
+Qed.
 
 Ltac inv_mbind :=
   repeat match goal with
@@ -397,209 +355,16 @@ Local Transparent gv2gvs.
 Opaque gv2gvs. 
 Qed.
 
-Lemma null_disjoint_with_ptr: forall td mb t,
-  mb > 0 ->
-  no_alias null ($ blk2GV td mb # typ_pointer t $).
-Proof.
-  intros. rewrite simpl_blk2GV. simpl. unfold Mem.nullptr.
-  repeat split; auto. intro. subst. omega.
-Qed.
-
-Lemma null_valid_ptrs: forall mb, mb > 0 -> valid_ptrs mb null.
-Proof.
-  intros. unfold null, Mem.nullptr. simpl. 
-  split; auto. omega.
-Qed.
-
-Lemma uninits_valid_ptrs: forall bd n, valid_ptrs bd (uninits n).
-Proof.
-  intros.
-  induction n; simpl; auto.
-Qed.
-
-Lemma uninits_disjoint_with_ptr: forall n td mb t,
-  no_alias (uninits n) ($ blk2GV td mb # typ_pointer t $).
-Proof.
-  intros.
-  rewrite simpl_blk2GV.
-  induction n; simpl; auto.
-Qed.
-
-Lemma uninits_valid_ptrs__disjoint_with_ptr: forall n td mb t bd,
-  no_alias (uninits n) ($ blk2GV td mb # typ_pointer t $) /\
-  valid_ptrs bd (uninits n).
-Proof.
-  intros.
-  split. apply uninits_disjoint_with_ptr.
-         apply uninits_valid_ptrs.
-Qed.
-
-Fixpoint no_embedded_ptrs (gvs:GenericValue): Prop :=
-match gvs with
-| nil => True
-| (Vptr _ _,_)::gvs' => False
-| _::gvs' => no_embedded_ptrs gvs'
-end.
-
-Lemma no_embedded_ptrs__no_alias_with_blk: forall b2 gvs1,
-  no_embedded_ptrs gvs1 -> no_alias_with_blk gvs1 b2.
-Proof.
-  induction gvs1 as [|[]]; simpl; intros; auto.
-    destruct v; auto. inv H.
-Qed.
-
-Lemma undef__no_embedded_ptrs: forall g td t1
-  (Hc2g : ret g = gundef td t1), no_embedded_ptrs g.
-Proof.
-  unfold gundef. intros.
-  inv_mbind'. simpl. auto.
-Qed.
-
-Lemma no_embedded_ptrs__no_alias: forall gvs1 gvs2,
-  no_embedded_ptrs gvs1 -> no_alias gvs1 gvs2.
-Proof.
-  induction gvs2 as [|[]]; simpl; intros; auto.
-    destruct v; auto.
-    split; auto using no_embedded_ptrs__no_alias_with_blk.
-Qed.
-
-Lemma undef_disjoint_with_ptr: forall g td t1 g'
-  (Hc2g : ret g = gundef td t1), no_alias g g'.
-Proof.
-  intros. apply undef__no_embedded_ptrs in Hc2g.
-  apply no_embedded_ptrs__no_alias; auto.
-Qed.
-
-Lemma no_alias_with_blk_app: forall g2 b g1,
-  no_alias_with_blk g1 b -> no_alias_with_blk g2 b -> 
-  no_alias_with_blk (g1++g2) b.
-Proof.
-  induction g1; simpl; intros; auto.
-    destruct a.
-    destruct v; auto.
-    destruct H; auto.
-Qed.
-
-Lemma no_alias_app: forall g2 g1 g,
-  no_alias g1 g -> no_alias g2 g -> no_alias (g1++g2) g.
-Proof.
-  induction g; simpl; intros; auto.
-    destruct a.
-    destruct v; auto.
-    destruct H. destruct H0.
-    split; auto using no_alias_with_blk_app.
-Qed.
-
-Lemma no_alias_nil: forall g, no_alias nil g.
-Proof.
-  induction g; simpl; intros; auto.
-    destruct a.
-    destruct v; auto.
-Qed.
-
-Lemma no_alias_repeatGV: forall g1 g2 n,
-  no_alias g1 g2 -> no_alias (repeatGV g1 n) g2.
-Proof.
-  induction n; simpl; intros.
-    apply no_alias_nil.
-    apply no_alias_app; auto.
-Qed.
-
-Lemma valid_ptrs_app: forall bd g2 g1,
-  valid_ptrs bd g1 -> valid_ptrs bd g2 -> valid_ptrs bd (g1++g2).
-Proof.
-  induction g1 as [|[]]; simpl; intros; auto.
-    destruct v; auto.
-    destruct H. 
-    split; auto.
-Qed.
-
-Lemma valid_ptrs_repeatGV: forall n bd g,
-  valid_ptrs bd g -> valid_ptrs bd (repeatGV g n).
-Proof.
-  induction n; simpl; intros; auto.
-    apply valid_ptrs_app; auto.
-Qed.
-
-Definition zeroconst2GV_disjoint_with_runtime_alloca_prop (t:typ) := 
-  forall maxb gl g td mb t0
-  (Hwfg: wf_globals maxb gl)
-  (Hc2g : ret g = zeroconst2GV td t)
-  (Hle: maxb < mb),
-  no_alias g ($ blk2GV td mb # typ_pointer t0 $) /\ valid_ptrs (maxb + 1) g.
-
-Definition zeroconsts2GV_disjoint_with_runtime_alloca_prop (lt:list_typ) := 
-  forall maxb gl g td mb t0
-  (Hwfg: wf_globals maxb gl)
-  (Hc2g : ret g = zeroconsts2GV td lt)
-  (Hle: maxb < mb),
-  no_alias g ($ blk2GV td mb # typ_pointer t0 $) /\ valid_ptrs (maxb + 1) g.
-
-Lemma zeroconst2GV_disjoint_with_runtime_alloca_mutrec :
-  (forall t, zeroconst2GV_disjoint_with_runtime_alloca_prop t) *
-  (forall lt, zeroconsts2GV_disjoint_with_runtime_alloca_prop lt).
-Proof.
-  apply typ_mutrec; 
-    unfold zeroconst2GV_disjoint_with_runtime_alloca_prop, 
-           zeroconsts2GV_disjoint_with_runtime_alloca_prop; 
-    intros; simpl in *;
-    try solve [inv Hc2g; rewrite simpl_blk2GV; simpl; auto].
-
-  destruct f; inv Hc2g; rewrite simpl_blk2GV; simpl; auto.
-
-  destruct s; 
-    try solve [inv Hc2g; auto using uninits_valid_ptrs__disjoint_with_ptr].
-    inv_mbind'.
-    eapply H with (t0:=t0) in HeqR; eauto.
-    assert (no_alias 
-      (g0 ++ uninits (Size.to_nat s0 - sizeGenericValue g0))
-      ($ blk2GV td mb # typ_pointer t0 $) /\
-      valid_ptrs (maxb + 1) 
-        (g0 ++ uninits (Size.to_nat s0 - sizeGenericValue g0))) as J.
-      destruct HeqR.
-      split.
-        apply no_alias_app; auto.
-          apply uninits_disjoint_with_ptr.
-        apply valid_ptrs_app; auto.
-          apply uninits_valid_ptrs.
-    destruct J as [J1 J2].
-    split.
-      apply no_alias_app; auto.
-      apply no_alias_repeatGV; auto.
-
-      apply valid_ptrs_app; auto.
-      apply valid_ptrs_repeatGV; auto.
-
-  inv_mbind'.
-  eapply H with (t0:=t0) in HeqR; eauto.
-  destruct g0; inv H1; auto.
-
-  inv Hc2g. 
-  split.
-    apply null_disjoint_with_ptr. destruct Hwfg. omega.
-    apply null_valid_ptrs. destruct Hwfg. omega.
-
-  inv_mbind'.
-  eapply H with (t0:=t0) in HeqR0; eauto.
-  eapply H0 with (t0:=t0) in HeqR; eauto.
-  destruct HeqR0. destruct HeqR.
-  split.
-    apply no_alias_app; auto.
-    apply no_alias_app; auto.
-    apply uninits_disjoint_with_ptr.
-
-    apply valid_ptrs_app; auto.
-    apply valid_ptrs_app; auto.
-    apply uninits_valid_ptrs.
-Qed.
-
 Lemma zeroconst2GV_disjoint_with_runtime_alloca: forall t maxb gl g td mb t0
   (Hwfg: wf_globals maxb gl)
   (Hc2g : ret g = zeroconst2GV td t)
   (Hle: maxb < mb),
   no_alias g ($ blk2GV td mb # typ_pointer t0 $) /\ valid_ptrs (maxb + 1) g.
 Proof.
-  destruct zeroconst2GV_disjoint_with_runtime_alloca_mutrec as [J _]; auto.
+  intros. rewrite simpl_blk2GV.
+  destruct zeroconst2GV_disjoint_with_runtime_ptr_mutrec as [J _].
+  unfold zeroconst2GV_disjoint_with_runtime_ptr_prop in J. 
+  eapply J; eauto.
 Qed.
 
 Tactic Notation "eapply_clear" hyp(H1) "in" hyp(H2) :=
@@ -608,759 +373,13 @@ Tactic Notation "eapply_clear" hyp(H1) "in" hyp(H2) :=
 Tactic Notation "apply_clear" hyp(H1) "in" hyp(H2) :=
   apply H1 in H2; auto; clear H1.
 
-Lemma wf_global_disjoint_with_runtime_alloca: forall maxb td t0
-  mb (Hle : maxb < mb) g0 (Hwfg : wf_global maxb g0),
-  no_alias g0 ($ blk2GV td mb # typ_pointer t0 $) /\ valid_ptrs (maxb + 1) g0.
-Proof.
-  induction g0 as [|[]]; simpl; intros.
-    split; auto using no_alias_nil.
-
-    destruct v; auto.
-      destruct Hwfg as [J1 J2].
-      apply_clear IHg0 in J2. rewrite simpl_blk2GV in *. 
-      simpl in *. destruct J2. destruct H.
-      split.
-        split; auto.    
-        split; auto. 
-          intro. subst. contradict J1. omega.
-
-        split; auto. omega.
-Qed.
-
 Lemma wf_globals_disjoint_with_runtime_alloca: forall maxb td t0
   (g0 : GenericValue) i0  mb (Hle : maxb < mb) gl (Hwfg : wf_globals maxb gl) 
   (HeqR : ret g0 = lookupAL GenericValue gl i0),
   no_alias g0 ($ blk2GV td mb # typ_pointer t0 $) /\ valid_ptrs (maxb + 1) g0.
 Proof.
-  induction gl as [|[]]; simpl; intros.
-    congruence.
-
-    destruct Hwfg. simpl in H0.
-    destruct H0 as [J1 J2].
-    destruct (i0 == i1); subst.
-      inv HeqR. eapply wf_global_disjoint_with_runtime_alloca; eauto.
-      apply IHgl; auto. split; auto.
-Qed.
-
-Lemma no_embedded_ptrs__valid_ptrs: forall bd gvs,
-  no_embedded_ptrs gvs -> valid_ptrs bd gvs.
-Proof.
-  induction gvs as [|[]]; simpl; intros; auto.
-    destruct v; auto.
-      inversion H.
-Qed.
-
-Lemma mtrunc_preserves_no_embedded_ptrs: forall td top t1 t2 gv gv',
-  mtrunc td top t1 t2 gv = Some gv' -> no_embedded_ptrs gv'.
-Proof.
-  intros.
-  unfold mtrunc in H.
-  remember (GV2val td gv) as R.
-  destruct R; eauto using undef__no_embedded_ptrs.
-  destruct v; eauto using undef__no_embedded_ptrs.
-    destruct t1; eauto using undef__no_embedded_ptrs.
-    destruct t2; eauto using undef__no_embedded_ptrs.
-      inv H. destruct (le_lt_dec wz s0); simpl; auto.
-
-    destruct t1; eauto using undef__no_embedded_ptrs.
-    destruct t2; eauto using undef__no_embedded_ptrs.
-    destruct (floating_point_order f1 f0); tinv H.
-    destruct f1; inv H; unfold val2GV; simpl; auto.
-Qed.
-
-Lemma mtrunc_preserves_no_alias: forall td top t1 t2 gv gv' gv0,
-  mtrunc td top t1 t2 gv = Some gv' -> no_alias gv' gv0.
-Proof.
-  intros.
-  apply no_embedded_ptrs__no_alias.
-  apply mtrunc_preserves_no_embedded_ptrs in H; auto.
-Qed.
-
-Lemma mtrunc_preserves_valid_ptrs: forall td top t1 t2 gv gv' bd,
-  mtrunc td top t1 t2 gv = Some gv' -> valid_ptrs bd gv'.
-Proof.
-  intros.
-  apply no_embedded_ptrs__valid_ptrs.
-  apply mtrunc_preserves_no_embedded_ptrs in H; auto.
-Qed.
-
-Lemma mext_preserves_no_embedded_ptrs: forall td eop t1 t2 gv gv',
-  mext td eop t1 t2 gv = Some gv' -> no_embedded_ptrs gv'.
-Proof.
-  intros.
-  unfold mext in H.
-  remember (GV2val td gv) as R.
-  destruct t1; tinv H.
-    destruct t2; tinv H.
-    destruct R; eauto using undef__no_embedded_ptrs.
-    destruct v; eauto using undef__no_embedded_ptrs.
-    destruct eop; inv H; simpl; auto.
-
-    destruct t2; tinv H.
-    destruct (floating_point_order f f0); tinv H.
-    destruct R; eauto using undef__no_embedded_ptrs.
-    destruct v; eauto using undef__no_embedded_ptrs.
-    destruct eop; tinv H; simpl; auto.
-    destruct f0; inv H; unfold val2GV; simpl; auto.
-Qed.
-
-Lemma mext_preserves_no_alias: forall td eop t1 t2 gv gv' gv0,
-  mext td eop t1 t2 gv = Some gv' -> no_alias gv' gv0.
-Proof.
-  intros.
-  apply no_embedded_ptrs__no_alias.
-  apply mext_preserves_no_embedded_ptrs in H; auto.
-Qed.
-
-Lemma mext_preserves_valid_ptrs: forall td eop t1 t2 gv gv' bd,
-  mext td eop t1 t2 gv = Some gv' -> valid_ptrs bd gv'.
-Proof.
-  intros.
-  apply no_embedded_ptrs__valid_ptrs.
-  apply mext_preserves_no_embedded_ptrs in H; auto.
-Qed.
-
-Lemma mbitcast_inv: forall t1 t2 gv1 gv2,
-  mbitcast t1 gv1 t2 = ret gv2 -> gv1 = gv2.
-Proof.
-  intros.
-  unfold mbitcast in H.
-  destruct t1; tinv H.
-    destruct t2; inv H; auto.
-    destruct t2; inv H; auto.
-Qed.
-
-Lemma mcast_inv: forall td cop t1 t2 gv1 gv2,
-  mcast td cop t1 t2 gv1 = ret gv2 -> gv2 = gv1 \/ gundef td t2 = ret gv2.
-Proof.
-  intros.
-  unfold mcast in H.
-  destruct cop; auto;
-    try 
-    match goal with
-    | H : mbitcast _ _ _ = ret _ |- _ => apply mbitcast_inv in H; subst; auto
-    end.
-Qed.
-
-Lemma mbitcast_preserves_no_alias: forall t1 t2 gv gv' gv0,
-  mbitcast t1 gv t2 = Some gv' ->
-  no_alias gv gv0 -> no_alias gv' gv0.
-Proof.
-  intros.
-  apply mbitcast_inv in H. subst. auto.
-Qed.
-
-Lemma mcast_preserves_no_alias: forall td cop t1 t2 gv gv' gv0,
-  mcast td cop t1 t2 gv = Some gv' ->
-  no_alias gv gv0 -> no_alias gv' gv0.
-Proof.
-  intros.
-  apply mcast_inv in H. 
-  destruct H as [H | H]; subst; eauto using undef_disjoint_with_ptr.
-Qed.
-
-Lemma undef_valid_ptrs: forall g td t1 blk
-  (Hc2g : ret g = gundef td t1), valid_ptrs blk g.
-Proof.
-  unfold gundef. intros.
-  inv_mbind'. simpl. auto.
-Qed.
-
-Lemma mcast_preserves_valid_ptrs: forall td cop t1 t2 gv gv' bd,
-  mcast td cop t1 t2 gv = Some gv' -> valid_ptrs bd gv -> valid_ptrs bd gv'.
-Proof.
-  intros.
-  apply mcast_inv in H. 
-  destruct H as [H | H]; subst; eauto using undef_valid_ptrs.
-Qed.
-
-Lemma no_alias_prop1: forall b i1 m1 i2 m2 g,
-  no_alias ((Vptr b i1, m1) :: nil) g -> no_alias ((Vptr b i2, m2) :: nil) g.
-Proof.
-  induction g as [|[]]; simpl; intros; auto.
-    destruct v; auto.
-    destruct H. simpl; auto.
-Qed.
-
-Lemma GV2ptr_inv: forall g1 td v,
-  ret v = GV2ptr td (getPointerSize td) g1 -> 
-  exists b, exists ofs, exists m, g1 = (Vptr b ofs, m)::nil /\ v = Vptr b ofs.
-Proof.
-  intros.
-  unfold GV2ptr in H.
-  destruct g1 as [|[]]; tinv H.
-  destruct v0; tinv H.
-  destruct g1 as [|[]]; inv H. 
-  unfold ptr2GV. unfold val2GV. eauto.
-Qed.
-
-Lemma GV2ptr_preserves_no_alias: forall g1 td g2 v,
-  no_alias g1 g2 ->
-  ret v = GV2ptr td (getPointerSize td) g1 ->
-  no_alias (ptr2GV td v) g2.
-Proof.
-  intros. apply GV2ptr_inv in H0. destruct H0 as [b [ofs [m [J1 J2]]]]; subst.
-  unfold ptr2GV. unfold val2GV. eapply no_alias_prop1; eauto.
-Qed.
-
-Lemma GV2ptr_preserves_valid_ptrs: forall bd g1 td v,
-  valid_ptrs bd g1 ->
-  ret v = GV2ptr td (getPointerSize td) g1 ->
-  valid_ptrs bd (ptr2GV td v).
-Proof.
-  intros. apply GV2ptr_inv in H0. destruct H0 as [b [ofs [m [J1 J2]]]]; subst.
-  unfold ptr2GV. unfold val2GV. simpl in *. auto.
-Qed.
-
-Lemma mgep_inv: forall td v1 t1 l1 v2,
-  ret v2 = mgep td t1 v1 l1 ->
-  exists b, exists ofs1, exists ofs2, v1 = Vptr b ofs1 /\ v2 = Vptr b ofs2.
-Proof.
-  intros.
-  unfold mgep in *.
-  destruct v1; tinv H.
-  destruct l1; tinv H.
-  destruct (mgetoffset td (typ_array 0%nat t1) (z :: l1)) as [[]|]; inv H.
-  eauto.
-Qed.  
-
-Lemma mgep_preserves_no_alias: forall td v t1 l1 v0 gv,
-  no_alias (ptr2GV td v) gv ->
-  ret v0 = mgep td t1 v l1 ->
-  no_alias (ptr2GV td v0) gv.
-Proof.
-  intros.
-  apply mgep_inv in H0. destruct H0 as [b [ofs1 [ofs2 [J1 J2]]]]; subst. 
-  unfold ptr2GV in *. unfold val2GV in *. eapply no_alias_prop1; eauto.
-Qed.
-
-Lemma mgep_preserves_valid_ptrs: forall td v t1 l1 v0 bd,
-  valid_ptrs bd (ptr2GV td v) ->
-  ret v0 = mgep td t1 v l1 ->
-  valid_ptrs bd (ptr2GV td v0).
-Proof.
-  intros.
-  apply mgep_inv in H0. destruct H0 as [b [ofs1 [ofs2 [J1 J2]]]]; subst. 
-  simpl in *. auto.
-Qed.
-
-Lemma nonptr_no_alias: forall v t td mb t0,
-  (forall b ofs, v <> Vptr b ofs) ->
-  no_alias (val2GV td v t) ($ blk2GV td mb # typ_pointer t0 $).
-Proof.
-  intros.
-  rewrite simpl_blk2GV.  
-  destruct v; simpl; auto.
-    assert (H1:=@H b i0). congruence.
-Qed.
-
-Lemma nonptr_no_embedded_ptrs: forall v t td,
-  (forall b ofs, v <> Vptr b ofs) -> no_embedded_ptrs (val2GV td v t).
-Proof.
-  intros.
-  destruct v; simpl; auto.
-    assert (H1:=@H b i0). congruence.
-Qed.
-
-Lemma micmp_int_preserves_no_embedded_ptrs: forall td cop gv1 gv2 gv',
-  micmp_int td cop gv1 gv2 = Some gv' -> no_embedded_ptrs gv'.
-Proof.
-  intros.
-  unfold micmp_int in H.
-  destruct (GV2val td gv1); eauto using undef__no_embedded_ptrs.
-  destruct v; eauto using undef__no_embedded_ptrs.
-  destruct (GV2val td gv2); eauto using undef__no_embedded_ptrs.
-  destruct v; eauto using undef__no_embedded_ptrs.
-Opaque Val.cmp Val.cmpu.
-  destruct cop; inv H;
-    apply nonptr_no_embedded_ptrs; 
-      try solve [auto | apply cmp_isnt_ptr | apply cmpu_isnt_ptr].
-Transparent Val.cmp Val.cmpu.
-Qed.
-
-Lemma micmp_int_preserves_no_alias: forall td cop gv1 gv2 gv' gv0,
-  micmp_int td cop gv1 gv2 = Some gv' -> no_alias gv' gv0.
-Proof.
-  intros.
-  apply no_embedded_ptrs__no_alias.
-  apply micmp_int_preserves_no_embedded_ptrs in H; auto.
-Qed.
-
-Lemma micmp_int_preserves_valid_ptrs: forall td cop gv1 gv2 bd gv',
-  micmp_int td cop gv1 gv2 = Some gv' -> valid_ptrs bd gv'.
-Proof.
-  intros.
-  apply no_embedded_ptrs__valid_ptrs.
-  apply micmp_int_preserves_no_embedded_ptrs in H; auto.
-Qed.
-
-Lemma micmp_preserves_no_alias: forall td cop t1 gv1 gv2 gv' gv0,
-  micmp td cop t1 gv1 gv2 = Some gv' -> no_alias gv' gv0.
-Proof.
-  intros.
-  unfold micmp in H.
-  destruct t1; tinv H; eauto using undef_disjoint_with_ptr.
-    eapply micmp_int_preserves_no_alias; eauto.
-Qed.
-
-Lemma micmp_preserves_valid_ptrs: forall td cop t1 gv1 gv2 gv' bd,
-  micmp td cop t1 gv1 gv2 = Some gv' -> valid_ptrs bd gv'.
-Proof.
-  intros.
-  unfold micmp in H.
-  destruct t1; tinv H; eauto using undef_valid_ptrs.
-    eapply micmp_int_preserves_valid_ptrs; eauto.
-Qed.
-
-Lemma mfcmp_preserves_no_alias: forall td fop fp gv1 gv2 gv' gv0,
-  mfcmp td fop fp gv1 gv2 = Some gv' -> no_alias gv' gv0.
-Proof.
-  intros.
-  unfold mfcmp in H.
-  destruct (GV2val td gv1); eauto using undef_disjoint_with_ptr.
-  destruct v; eauto using undef_disjoint_with_ptr.
-  destruct (GV2val td gv2); eauto using undef_disjoint_with_ptr.
-  destruct v; eauto using undef_disjoint_with_ptr.
-  apply no_embedded_ptrs__no_alias.
-  destruct fp; tinv H;
-    destruct fop; inv H; apply nonptr_no_embedded_ptrs; 
-      try solve [auto | apply Vfalse_isnt_ptr | apply Vtrue_isnt_ptr | 
-                 apply val_of_bool_isnt_ptr].
-Qed.
-
-Lemma mfcmp_preserves_valid_ptrs: forall td fop fp gv1 gv2 gv' bd,
-  mfcmp td fop fp gv1 gv2 = Some gv' -> valid_ptrs bd gv'.
-Proof.
-  intros.
-  unfold mfcmp in H.
-  destruct (GV2val td gv1); eauto using undef_valid_ptrs.
-  destruct v; eauto using undef_valid_ptrs.
-  destruct (GV2val td gv2); eauto using undef_valid_ptrs.
-  destruct v; eauto using undef_valid_ptrs.
-  apply no_embedded_ptrs__valid_ptrs.
-  destruct fp; tinv H;
-    destruct fop; inv H; apply nonptr_no_embedded_ptrs; 
-      try solve [auto | apply Vfalse_isnt_ptr | apply Vtrue_isnt_ptr | 
-                 apply val_of_bool_isnt_ptr].
-Qed.
-
-Lemma no_alias_with_blk_split: forall g2 b g1,
-  no_alias_with_blk (g1++g2) b -> 
-  no_alias_with_blk g1 b /\ no_alias_with_blk g2 b.
-Proof.
-  induction g1 as [|[]]; simpl; intros; auto.
-    destruct v; auto.
-    destruct H. apply IHg1 in H0. destruct H0. split; auto.
-Qed.
-
-Lemma no_alias_split: forall g2 g1 g,
-  no_alias (g1++g2) g -> no_alias g1 g /\ no_alias g2 g.
-Proof.
-  induction g as [|[]]; simpl; intros; auto.
-    destruct v; auto.
-
-    destruct H. apply IHg in H0. destruct H0.
-    apply no_alias_with_blk_split in H. destruct H.
-    repeat split; auto.
-Qed.
-
-Lemma valid_ptrs_split: forall bd g2 g1,
-  valid_ptrs bd (g1++g2) -> valid_ptrs bd g1 /\ valid_ptrs bd g2.
-Proof.
-  induction g1 as [|[]]; simpl; intros; auto.
-    destruct v; auto.
-    destruct H. apply IHg1 in H0. destruct H0.
-    repeat split; auto.
-Qed.
-
-Lemma splitGenericValue_preserves_no_alias: forall gv g0 z0 g1 g2,
-  no_alias g0 gv ->
-  ret (g1, g2) = splitGenericValue g0 z0 ->
-  no_alias g1 gv /\ no_alias g2 gv.
-Proof.
-  induction g0 as [|[]]; simpl; intros.
-    destruct (zeq z0 0).
-      inv H0. split; apply no_alias_nil.
-      destruct (zlt z0 0); tinv H0.
-
-    destruct (zeq z0 0).
-      inv H0. split; auto using no_alias_nil.
-
-      destruct (zlt z0 0); tinv H0.
-      inv_mbind'. inv H2.
-      simpl_env in H.
-      apply no_alias_split in H; auto.
-      destruct H.
-      apply IHg0 in HeqR; auto.
-      destruct HeqR. split; auto.
-      simpl_env. apply no_alias_app; auto.
-Qed.
-
-Lemma splitGenericValue_preserves_valid_ptrs: forall bd g0 z0 g1 g2,
-  valid_ptrs bd g0 ->
-  ret (g1, g2) = splitGenericValue g0 z0 ->
-  valid_ptrs bd g1 /\ valid_ptrs bd g2.
-Proof.
-  induction g0 as [|[]]; simpl; intros.
-    destruct (zeq z0 0).
-      inv H0. auto.
-      destruct (zlt z0 0); tinv H0.
-
-    destruct (zeq z0 0).
-      inv H0. simpl. auto.
-
-      destruct (zlt z0 0); tinv H0.
-      inv_mbind'. inv H2.
-      simpl_env in H.
-      assert (valid_ptrs bd [(v,m)] /\ valid_ptrs bd g0) as J.
-        simpl. 
-        destruct v; auto.
-          destruct H; auto.
-      destruct J as [J1 J2].
-      apply IHg0 in HeqR; auto.
-      destruct HeqR. 
-      split; auto.
-        simpl_env.
-        apply valid_ptrs_app; auto.
-Qed.
-
-Lemma extractGenericValue_preserves_no_alias: forall td gv t1 g0 g1 l0,
-  no_alias g0 gv -> ret g1 = extractGenericValue td t1 g0 l0 -> no_alias g1 gv.
-Proof.
-  intros.
-  unfold extractGenericValue in *.
-  inv_mbind'.
-  remember (mget td g0 z t) as R.
-  destruct R; eauto using undef_disjoint_with_ptr.
-  inv H1.
-  unfold mget in HeqR1.
-  destruct (getTypeStoreSize td t); tinv HeqR1.
-  simpl in HeqR1.
-  inv_mbind'. inv H2.
-  eapply splitGenericValue_preserves_no_alias in HeqR2; eauto.
-  destruct HeqR2.
-  eapply splitGenericValue_preserves_no_alias in HeqR1; eauto.
-  destruct HeqR1; auto.
-Qed.
-
-Lemma extractGenericValue_preserves_valid_ptrs: forall td g1 t1 g0 bd l0,
-  valid_ptrs bd g0 -> ret g1 = extractGenericValue td t1 g0 l0 -> 
-  valid_ptrs bd g1.
-Proof.
-  intros.
-  unfold extractGenericValue in *.
-  inv_mbind'.
-  remember (mget td g0 z t) as R.
-  destruct R; eauto using undef_valid_ptrs.
-  inv H1.
-  unfold mget in HeqR1.
-  destruct (getTypeStoreSize td t); tinv HeqR1.
-  simpl in HeqR1.
-  inv_mbind'. inv H2.
-  eapply splitGenericValue_preserves_valid_ptrs in HeqR2; eauto.
-  destruct HeqR2.
-  eapply splitGenericValue_preserves_valid_ptrs in HeqR1; eauto.
-  destruct HeqR1; auto.
-Qed.
-
-Lemma insertGenericValue_preserves_no_alias: forall td gv t1 t2 g0 g1 g2 l0,
-  no_alias g0 gv -> no_alias g1 gv ->
-  ret g2 = insertGenericValue td t1 g0 l0 t2 g1 -> no_alias g2 gv.
-Proof.
-  intros.
-  unfold insertGenericValue in *.
-  inv_mbind'.
-  remember (mset td g0 z t2 g1) as R.
-  destruct R; eauto using undef_disjoint_with_ptr.
-  inv H2.
-  unfold mset in HeqR1.
-  destruct (getTypeStoreSize td t2); tinv HeqR1.
-  simpl in HeqR1.
-  destruct (n =n= length g1); tinv HeqR1.
-  inv_mbind'. inv H3.
-  eapply splitGenericValue_preserves_no_alias in HeqR2; eauto.
-  destruct HeqR2.
-  eapply splitGenericValue_preserves_no_alias in HeqR1; eauto.
-  destruct HeqR1.
-  repeat apply no_alias_app; auto.
-Qed.
-
-Lemma insertGenericValue_preserves_valid_ptrs: forall td t1 t2 g0 g1 g2 l0 bd,
-  valid_ptrs bd g0 -> valid_ptrs bd g1 ->
-  ret g2 = insertGenericValue td t1 g0 l0 t2 g1 -> valid_ptrs bd g2.
-Proof.
-  intros.
-  unfold insertGenericValue in *.
-  inv_mbind'.
-  remember (mset td g0 z t2 g1) as R.
-  destruct R; eauto using undef_valid_ptrs.
-  inv H2.
-  unfold mset in HeqR1.
-  destruct (getTypeStoreSize td t2); tinv HeqR1.
-  simpl in HeqR1.
-  destruct (n =n= length g1); tinv HeqR1.
-  inv_mbind'. inv H3.
-  eapply splitGenericValue_preserves_valid_ptrs in HeqR2; eauto.
-  destruct HeqR2.
-  eapply splitGenericValue_preserves_valid_ptrs in HeqR1; eauto.
-  destruct HeqR1.
-  repeat apply valid_ptrs_app; auto.
-Qed.
-
-Lemma mbop_preserves_no_embedded_ptrs: forall td bop0 sz0 gv1 gv2 gv3,
-  mbop td bop0 sz0 gv1 gv2 = Some gv3 -> no_embedded_ptrs gv3.
-Proof.
-  intros.
-  unfold mbop in H.
-  destruct (GV2val td gv1); eauto using undef__no_embedded_ptrs.
-  destruct v; eauto using undef__no_embedded_ptrs.
-  destruct (GV2val td gv2); eauto using undef__no_embedded_ptrs.
-  destruct v; eauto using undef__no_embedded_ptrs.
-  destruct (eq_nat_dec (wz + 1) (Size.to_nat sz0)); 
-    eauto using undef__no_embedded_ptrs.
-  destruct bop0; inv H;
-    apply nonptr_no_embedded_ptrs;
-      try solve [apply add_isnt_ptr | apply sub_isnt_ptr | apply mul_isnt_ptr |
-                 apply divu_isnt_ptr | apply divs_isnt_ptr | apply modu_isnt_ptr |
-                 apply mods_isnt_ptr | apply shl_isnt_ptr | apply shrx_isnt_ptr |
-                 apply shr_isnt_ptr | apply and_isnt_ptr | apply or_isnt_ptr |
-                 apply xor_isnt_ptr].
-Qed.
-
-Lemma mbop_preserves_no_alias: forall td bop0 sz0 gv1 gv2 gv3 gv,
-  mbop td bop0 sz0 gv1 gv2 = Some gv3 ->
-  no_alias gv3 gv.
-Proof.
-  intros.
-  apply no_embedded_ptrs__no_alias.
-  apply mbop_preserves_no_embedded_ptrs in H; auto.
-Qed.
-
-Lemma mbop_preserves_valid_ptrs: forall td bop0 sz0 gv1 gv2 gv3 bd,
-  mbop td bop0 sz0 gv1 gv2 = Some gv3 ->
-  valid_ptrs bd gv3.
-Proof.
-  intros.
-  apply no_embedded_ptrs__valid_ptrs.
-  apply mbop_preserves_no_embedded_ptrs in H; auto.
-Qed.
-
-Lemma mfbop_preserves_no_embedded_ptrs: forall td fbop0 fp0 gv1 gv2 gv3,
-  mfbop td fbop0 fp0 gv1 gv2 = Some gv3 -> no_embedded_ptrs gv3.
-Proof.
-  intros.
-  unfold mfbop in H.
-  destruct (GV2val td gv1); eauto using undef__no_embedded_ptrs.
-  destruct v; eauto using undef__no_embedded_ptrs.
-  destruct (GV2val td gv2); eauto using undef__no_embedded_ptrs.
-  destruct v; eauto using undef__no_embedded_ptrs.
-  destruct fp0; tinv H; destruct fbop0; inv H; simpl; auto.
-Qed.
-
-Lemma mfbop_preserves_no_alias: forall td fbop0 fp0 gv1 gv2 gv3 gv0,
-  mfbop td fbop0 fp0 gv1 gv2 = Some gv3 -> no_alias gv3 gv0.
-Proof.
-  intros.
-  apply no_embedded_ptrs__no_alias.
-  apply mfbop_preserves_no_embedded_ptrs in H; auto.
-Qed.
-
-Lemma mfbop_preserves_valid_ptrs: forall td fbop0 fp0 gv1 gv2 gv3 bd,
-  mfbop td fbop0 fp0 gv1 gv2 = Some gv3 -> valid_ptrs bd gv3.
-Proof.
-  intros.
-  apply no_embedded_ptrs__valid_ptrs.
-  apply mfbop_preserves_no_embedded_ptrs in H; auto.
-Qed.
-
-Lemma undef_valid_ptrs__disjoint_with_ptr: forall g td t1 blk g'
-  (Hc2g : ret g = gundef td t1), no_alias g g' /\ valid_ptrs blk g.
-Proof.
-  intros.
-  split.
-    eapply undef_disjoint_with_ptr; eauto.
-    eapply undef_valid_ptrs; eauto.
-Qed.
-
-Definition const2GV_disjoint_with_runtime_alloca_prop (c:const) := 
-  forall maxb gl g td mb t t0
-  (Hwfg: wf_globals maxb gl)
-  (Hc2g : ret (g, t0) = _const2GV td gl c)
-  (Hle: maxb < mb),
-  no_alias g ($ blk2GV td mb # typ_pointer t $) /\ valid_ptrs (maxb+1) g.
-
-Definition list_const2GV_disjoint_with_runtime_alloca_prop (lc:list_const) :=
-  forall maxb gl td mb t
-  (Hwfg: wf_globals maxb gl)
-  (Hle: maxb < mb),
-  (forall gv, 
-    _list_const_arr2GV td gl t lc = Some gv ->
-    no_alias gv ($ blk2GV td mb # typ_pointer t $) /\ valid_ptrs (maxb+1) gv
-  ) /\
-  (forall gv t0, 
-    _list_const_struct2GV td gl lc = Some (gv,t0) ->
-    no_alias gv ($ blk2GV td mb # typ_pointer t $) /\ valid_ptrs (maxb+1) gv
-  ).
-
-Lemma const2GV_disjoint_with_runtime_alloca_mutrec :
-  (forall c, const2GV_disjoint_with_runtime_alloca_prop c) *
-  (forall lc, list_const2GV_disjoint_with_runtime_alloca_prop lc).
-Proof.
-  apply const_mutrec; 
-    unfold const2GV_disjoint_with_runtime_alloca_prop, 
-           list_const2GV_disjoint_with_runtime_alloca_prop;
-    intros; simpl in *; eauto; inv_mbind'.
-Case "zero".
-  eapply zeroconst2GV_disjoint_with_runtime_alloca; eauto.
-Case "int".
-  rewrite simpl_blk2GV. inv Hc2g. simpl. auto.
-Case "float".
-  rewrite simpl_blk2GV. destruct f; inv Hc2g; simpl; auto.
-Case "undef".
-  eapply undef_valid_ptrs__disjoint_with_ptr with (t1:=t)(td:=td); auto.
-Case "null".
-  inv Hc2g. simpl. 
-  destruct Hwfg. 
-  split.
-    apply null_disjoint_with_ptr. omega.
-    apply null_valid_ptrs. omega.
-Case "arr". 
-  eapply H with (td:=td)(gl:=gl)(t:=t) in Hle; eauto.
-  destruct Hle.
-  destruct (length (unmake_list_const l0)); inv H1; 
-    eauto using uninits_valid_ptrs__disjoint_with_ptr.
-Case "struct". 
-  eapply H with (td:=td)(gl:=gl)(t:=t) in Hle; eauto.
-  destruct Hle. 
-  destruct g0; inv H1; 
-    eauto using uninits_valid_ptrs__disjoint_with_ptr.
-Case "gid".
-  eapply wf_globals_disjoint_with_runtime_alloca; eauto.
-Case "trunc". 
-  split. 
-    eapply mtrunc_preserves_no_alias; eauto.
-    eapply mtrunc_preserves_valid_ptrs; eauto.
-Case "ext". 
-  split. 
-    eapply mext_preserves_no_alias; eauto.
-    eapply mext_preserves_valid_ptrs; eauto.
-Case "cast". 
-  eapply H in HeqR; eauto. destruct HeqR.
-  split.
-    eapply mcast_preserves_no_alias; eauto.
-    eapply mcast_preserves_valid_ptrs; eauto.
-Case "gep". 
-  destruct t1; tinv H2. 
-  inv_mbind'.
-  remember (GV2ptr td (getPointerSize td) g0) as R1.
-  remember (gundef td t2) as R3.
-  destruct R1.
-    destruct (intConsts2Nats td l0).
-      remember (mgep td t1 v l1) as R2.
-      destruct R2.
-        inv H3. 
-        eapply H with (t:=t) in HeqR; eauto.
-        destruct HeqR as [J1 J2].
-        split.
-          eapply GV2ptr_preserves_no_alias in HeqR1; eauto.
-          eapply mgep_preserves_no_alias; eauto.
-
-          eapply GV2ptr_preserves_valid_ptrs in HeqR1; eauto.
-          eapply mgep_preserves_valid_ptrs; eauto.
-
-        destruct R3; inv H3; eauto using undef_valid_ptrs__disjoint_with_ptr.
-      destruct R3; inv H3; eauto using undef_valid_ptrs__disjoint_with_ptr.
-    destruct R3; inv H3; eauto using undef_valid_ptrs__disjoint_with_ptr.
-
-Case "select". destruct (isGVZero td g0); inv H3; eauto.
-Case "icmp". 
-  split.
-    eapply micmp_preserves_no_alias; eauto.
-    eapply micmp_preserves_valid_ptrs; eauto.
-Case "fcmp". 
-  destruct t1; tinv H2. inv_mbind'.
-  split.
-    eapply mfcmp_preserves_no_alias; eauto.
-    eapply mfcmp_preserves_valid_ptrs; eauto.
-Case "extractValue". 
-  eapply H in HeqR; eauto.
-  destruct HeqR.
-  split.
-    eapply extractGenericValue_preserves_no_alias in HeqR1; eauto.
-    eapply extractGenericValue_preserves_valid_ptrs in HeqR1; eauto.
-Case "insertValue". 
-  eapply H with (t:=t) in HeqR; eauto. clear H.
-  eapply H0 with (t:=t) in HeqR0; eauto. clear H0 H1.
-  destruct HeqR. destruct HeqR0.
-  split.
-    eapply insertGenericValue_preserves_no_alias in HeqR1; eauto.
-    eapply insertGenericValue_preserves_valid_ptrs in HeqR1; eauto.
-Case "bop". 
-  destruct t1; tinv H2. inv_mbind'.
-  split.
-    eapply mbop_preserves_no_alias; eauto.
-    eapply mbop_preserves_valid_ptrs; eauto.
-Case "fbop". 
-  destruct t1; tinv H2. inv_mbind'.
-  split.
-    eapply mfbop_preserves_no_alias; eauto.
-    eapply mfbop_preserves_valid_ptrs; eauto.
-Case "nil".
-  split.
-    intros gv J. inv J. simpl. auto using no_alias_nil.
-    intros gv t0 J. inv J. simpl. auto using no_alias_nil.
-Case "cons".
-  split; intros; inv_mbind'. 
-    destruct p. 
-    destruct (typ_dec t t0); tinv H2.
-    inv_mbind'.
-    eapply H with (t:=t0) in HeqR0; eauto.
-    eapply H0 with (t:=t0)(td:=td) in Hwfg; eauto.
-    destruct Hwfg. symmetry in HeqR. apply H1 in HeqR.
-    destruct HeqR0. destruct HeqR.
-    split.
-      apply no_alias_app.
-        apply no_alias_app; auto.
-        apply uninits_disjoint_with_ptr.
-      apply valid_ptrs_app.
-        apply valid_ptrs_app; auto.
-        apply uninits_valid_ptrs.
-
-    destruct p. inv_mbind'. 
-    destruct p. inv_mbind'. 
-    eapply H with (t:=t) in HeqR0; eauto.
-    eapply H0 with (t:=t)(td:=td) in Hwfg; eauto.
-    destruct Hwfg. symmetry in HeqR. apply H2 in HeqR.
-    destruct HeqR0. destruct HeqR.
-    split.
-      apply no_alias_app; auto.
-      apply no_alias_app; auto.
-      apply uninits_disjoint_with_ptr.
-
-      apply valid_ptrs_app; auto.
-      apply valid_ptrs_app; auto.
-      apply uninits_valid_ptrs.
-Qed.
-
-Lemma cgv2gvs_preserves_no_alias: forall g0 td mb t t0 maxb,
-  no_alias g0 ($ blk2GV td mb # typ_pointer t $) ->
-  0 <= maxb < mb ->
-  no_alias (cgv2gvs DGVs g0 t0) ($ blk2GV td mb # typ_pointer t $).
-Proof.
-  intros.
-Local Transparent cgv2gvs.
-  unfold cgv2gvs. simpl. unfold MDGVs.cgv2gvs. unfold cgv2gv.
-  destruct g0 as [|[]]; auto.
-  destruct v; auto.
-  destruct g0 as [|]; auto.
-
-  unfold cundef_gv.
-  rewrite simpl_blk2GV.
-  destruct t0; auto.
-    destruct f; auto.
-
-    rewrite <- simpl_blk2GV with (t:=t0).
-    apply null_disjoint_with_ptr. omega.
+  intros. rewrite simpl_blk2GV. 
+  eapply wf_globals_disjoint_with_runtime_ptr; eauto.
 Qed.
 
 Lemma const2GV_disjoint_with_runtime_alloca: forall c0 maxb gl g td mb t
@@ -1372,28 +391,13 @@ Proof.
   unfold Opsem.const2GV.
   intros.
   inv_mbind'. inv H0.
-  destruct const2GV_disjoint_with_runtime_alloca_mutrec as [J1 J2].
-  unfold const2GV_disjoint_with_runtime_alloca_prop in J1. 
-  eapply J1 with (t:=t) in HeqR; eauto.
+  destruct const2GV_disjoint_with_runtime_ptr_mutrec as [J1 J2].
+  unfold const2GV_disjoint_with_runtime_ptr_prop in J1. 
+  rewrite simpl_blk2GV.
+  eapply J1 in HeqR; eauto.
   destruct HeqR. 
   destruct Hwfg.
   eapply cgv2gvs_preserves_no_alias; eauto.
-Qed.
-
-Lemma cgv2gvs_preserves_valid_ptrs: forall g0 t0 bd,
-  bd > 0 -> valid_ptrs bd g0 -> valid_ptrs bd (cgv2gvs DGVs g0 t0).
-Proof.
-  intros.
-Local Transparent cgv2gvs.
-  unfold cgv2gvs. simpl. unfold MDGVs.cgv2gvs. unfold cgv2gv.
-  destruct g0 as [|[]]; auto.
-  destruct v; auto.
-  destruct g0 as [|]; auto.
-  unfold cundef_gv.
-  destruct t0; auto.
-    destruct f; auto.
-
-    apply null_valid_ptrs; auto.
 Qed.
 
 Lemma const2GV_valid_ptrs: forall c0 maxb gl g td 
@@ -1404,9 +408,11 @@ Proof.
   unfold Opsem.const2GV.
   intros.
   inv_mbind'. inv H0.
-  destruct const2GV_disjoint_with_runtime_alloca_mutrec as [J1 J2].
-  unfold const2GV_disjoint_with_runtime_alloca_prop in J1. 
-  eapply J1 with (t:=t)(mb:=maxb+1) in HeqR; eauto; try omega.
+  destruct const2GV_disjoint_with_runtime_ptr_mutrec as [J1 J2].
+  unfold const2GV_disjoint_with_runtime_ptr_prop in J1. 
+  eapply J1 with (mb:=maxb+1)(ofs:=Int.repr 31 0)
+    (m:=AST.Mint (Size.mul Size.Eight (getPointerSize td) - 1)) in HeqR; 
+    eauto; try omega.
   destruct HeqR. 
   destruct Hwfg.
   eapply cgv2gvs_preserves_valid_ptrs; eauto; try omega.
@@ -1453,78 +459,8 @@ Proof.
     eapply undef_disjoint_with_ptr; eauto.
 Qed.
 
-Lemma wf_als_split: forall maxb M als als',
-  wf_als maxb M (als++als') -> wf_als maxb M als /\ wf_als maxb M als'.
-Proof.
-  intros.
-  destruct H as [J1 J2].
-  apply NoDup_split in J1.
-  destruct J1 as [J11 J12].
-  split.
-    split; auto.
-      intros. apply J2. apply in_or_app; auto.
-    split; auto.
-      intros. apply J2. apply in_or_app; auto.
-Qed.
-
 Ltac SSSSSCase name := Case_aux subsubsubsubsubcase name.
 Ltac SSSSSSCase name := Case_aux subsubsubsubsubsubcase name.
-
-Lemma load_free': forall (blk : Values.block) (lo : Z) (hi : Z) 
-  (b : Values.block) (Mem : Memory.mem) (Mem' : Memory.mem)
-  (Hfree : Mem.free Mem blk lo hi = ret Mem')
-  (a : AST.memory_chunk) (ofs : Z) (v : val)
-  (HeqR : ret v = Mem.load a Mem' b ofs),
-  b <> blk \/ lo >= hi \/ ofs + size_chunk a <= lo \/ hi <= ofs.
-Proof.
-  intros.
-  symmetry in HeqR.
-  apply Mem.load_valid_access in HeqR.
-  destruct (zeq b blk); subst; auto.
-  right.
-  destruct (zlt lo hi); try omega.
-  destruct (zle (ofs + size_chunk a) lo); auto.
-  destruct (zle hi ofs); auto.
-  contradict HeqR.
-  eapply Mem.valid_access_free_2 in Hfree; eauto; try omega.
-Qed.      
-
-Lemma free_preserves_mload_aux_inv: forall blk lo hi b Mem Mem' 
-  (Hfree:Mem.free Mem blk lo hi = ret Mem') mc ofs gvsa,
-  mload_aux Mem' mc b ofs = ret gvsa ->
-  mload_aux Mem mc b ofs = ret gvsa.
-Proof.
-  induction mc; simpl; intros; auto.
-    inv_mbind'. symmetry in HeqR0.
-    apply IHmc in HeqR0.
-    rewrite HeqR0.
-    erewrite <- Mem.load_free; eauto.
-      rewrite <- HeqR. auto.
-      eapply load_free'; eauto.
-Qed.
-
-Lemma free_preserves_mload_inv: forall TD Mem' gptr ty al gvsa Mem mptr0
-  (H1 : mload TD Mem' gptr ty al = ret gvsa)
-  (H2 : free TD Mem mptr0 = ret Mem'),
-  mload TD Mem gptr ty al = ret gvsa.
-Proof.
-  intros.
-  apply mload_inv in H1.
-  destruct H1 as [b [ofs [m [mc [J1 [J2 J3]]]]]]; subst.
-  unfold mload. simpl. rewrite J2.
-  apply free_inv in H2.
-  destruct H2 as [blk' [ofs' [hi [lo [J4 [J5 [J6 J7]]]]]]].
-  eapply free_preserves_mload_aux_inv; eauto.
-Qed.
-
-Lemma nextblock_free: forall TD M gv M', 
-  free TD M gv = ret M' -> Mem.nextblock M = Mem.nextblock M'.
-Proof.  
-  intros.
-  apply free_inv in H.
-  destruct H as [blk' [ofs' [hi [lo [J4 [J5 [J6 J7]]]]]]].
-  apply Mem.nextblock_free in J7. auto.
-Qed.
 
 Lemma free_preserves_wf_ECStack_head_tail : forall maxb pinfo TD M M' lc mptr0
   (Hfree: free TD M mptr0 = ret M') ECs 
@@ -1542,52 +478,6 @@ Proof.
   split; auto.
     intros.
     eapply free_preserves_mload_inv in H; eauto.
-Qed.
-
-Lemma free_preserves_wf_lc: forall TD Mem' Mem mptr0
-  (H2 : free TD Mem mptr0 = ret Mem') lc
-  (Hwf: wf_lc Mem lc),
-  wf_lc Mem' lc.
-Proof.
-  unfold wf_lc.
-  intros.
-  apply Hwf in H.
-  apply free_inv in H2.
-  destruct H2 as [blk' [ofs' [hi [lo [J4 [J5 [J6 J7]]]]]]].
-  erewrite Mem.nextblock_free; eauto.
-Qed.
-
-Lemma free_preserves_mload_aux: forall Mem blk lo hi Mem' b
-  (Hfree: Mem.free Mem blk lo hi = ret Mem') (Hneq: blk <> b) mc ofs gv,
-  mload_aux Mem mc b ofs = ret gv ->
-  mload_aux Mem' mc b ofs = ret gv.
-Proof.
-  induction mc; simpl; intros; auto.
-    inv_mbind'. symmetry in HeqR0.
-    apply IHmc in HeqR0.
-    rewrite HeqR0.
-    erewrite Mem.load_free; eauto.
-      rewrite <- HeqR. auto.
-Qed.
-
-Lemma free_preserves_mload: forall TD Mem Mem' t al gv gptr gvsa
-  (H0 : no_alias gptr gvsa)
-  (H1 : free TD Mem gptr = ret Mem')
-  (H2 : mload TD Mem gvsa t al = ret gv),
-  mload TD Mem' gvsa t al = ret gv.
-Proof.
-  intros.
-  apply free_inv in H1.
-  destruct H1 as [blk [ofs [hi [lo [J4 [J5 [J6 J7]]]]]]].
-  apply mload_inv in H2.
-  destruct H2 as [b [ofs' [m [mc [J1 [J2 J3]]]]]]; subst.
-  unfold mload. simpl. rewrite J2.
-  symmetry in J4.
-  apply GV2ptr_inv in J4.
-  destruct J4 as [b1 [ofs1 [m1 [J8 J9]]]]; subst.
-  inv J9.
-  simpl in H0. destruct H0. destruct H. clear H1 H0.
-  eapply free_preserves_mload_aux in J3; eauto.
 Qed.
 
 Lemma operand__no_alias_with__tail: forall maxb pinfo TD M lc1 lc2 mptr0 gl
@@ -1760,43 +650,6 @@ Proof.
 (* Can this lemma be more generic by making free_preserves_mload_inv generic? *)
 Qed.
 
-Lemma free_preserves_wf_Mem : forall maxb TD M M' mptr0
-  (Hfree: free TD M mptr0 = ret M') 
-  (Hwf: wf_Mem maxb TD M),
-  wf_Mem maxb TD M'.
-Proof.
-  intros. destruct Hwf as [J1 J2].
-  unfold wf_Mem.
-  erewrite <- nextblock_free; eauto.
-  split; auto.
-    intros. 
-    eapply free_preserves_mload_inv in H; eauto.
-Qed.
-
-Lemma free_preserves_wf_als : forall maxb TD M M' mptr0 als
-  (Hfree: free TD M mptr0 = ret M') 
-  (Hwf: wf_als maxb M als),
-  wf_als maxb M' als.
-Proof.
-  intros. destruct Hwf as [J1 J2].
-  split; auto.
-    intros. 
-    apply J2 in H.
-    erewrite <- nextblock_free; eauto.
-Qed.
-
-Lemma free_allocas_preserves_mload_inv: forall TD gptr ty al gvsa als Mem' Mem
-  (H1 : mload TD Mem' gptr ty al = ret gvsa)
-  (H2 : free_allocas TD Mem als = ret Mem'),
-  mload TD Mem gptr ty al = ret gvsa.
-Proof.
-  induction als; simpl; intros.
-    inv H2. auto.
-
-    inv_mbind.
-    eapply free_preserves_mload_inv with (Mem':=m); eauto.
-Qed.
-
 Lemma free_allocas_preserves_mload: forall TD al t mb gv als Mem' Mem 
   (H0 : ~ In mb als)
   (H1 : free_allocas TD Mem als = ret Mem')
@@ -1806,24 +659,13 @@ Proof.
   induction als; simpl; intros.
     inv H1. auto.
 
-    inv_mbind.
+    inv_mbind'.
     apply IHals in H3; auto.
     eapply free_preserves_mload; eauto.
     unfold_blk2GV. 
 Local Transparent gv2gvs.
   unfold gv2gvs. simpl. split; auto.
 Opaque gv2gvs. 
-Qed.
-
-Lemma nextblock_free_allocas: forall TD als M M', 
-  free_allocas TD M als = ret M' -> Mem.nextblock M = Mem.nextblock M'.
-Proof.  
-  induction als; simpl; intros.  
-    inv H. auto.
-
-    inv_mbind'. symmetry in HeqR.
-    apply nextblock_free in HeqR; auto.
-    rewrite HeqR. auto.
 Qed.
 
 Lemma free_allocas_preserves_wf_alloca: forall maxb pinfo TD Mem gvsa als0 als Mem',
@@ -1858,36 +700,6 @@ Proof.
   apply H in Hlkp; auto. clear H.
   destruct Hlkp as [J1 J2]. 
   split; eauto using free_allocas_preserves_wf_alloca.
-Qed.
-
-Lemma free_allocas_preserves_wf_lc: forall td lc als Mem Mem',
-  free_allocas td Mem als = ret Mem' -> wf_lc Mem lc -> wf_lc Mem' lc.
-Proof.
-  induction als; simpl; intros.
-    inv H. auto.
-
-    inv_mbind. symmetry in HeqR.
-    eapply free_preserves_wf_lc in HeqR; eauto.
-Qed.
-
-Lemma updateAddAL__wf_lc: forall gv3 Mem0 lc id0
-  (Hwfgv: valid_ptrs (Mem.nextblock Mem0) gv3) (Hwflc: wf_lc Mem0 lc),
-  wf_lc Mem0 (updateAddAL (GVsT DGVs) lc id0 gv3).
-Proof.
-  intros. unfold wf_lc in *. intros.
-  destruct (id_dec id0 id1); subst.
-    rewrite lookupAL_updateAddAL_eq in H. inv H. eauto.
-
-    rewrite <- lookupAL_updateAddAL_neq in H; auto.
-    eapply Hwflc; eauto.
-Qed.
-
-Lemma valid_ptrs__trans: forall bound1 bound2 gv,
-  valid_ptrs bound1 gv -> bound1 <= bound2 -> valid_ptrs bound2 gv.
-Proof.
-  induction gv as [|[]]; simpl; intros; auto.
-    destruct v; auto.
-      destruct H. split; auto. omega.
 Qed.
 
 Lemma operand__lt_nextblock: forall maxb TD M (lc:DGVMap) mptr gl
@@ -2086,31 +898,6 @@ Proof.
 Local Transparent gv2gvs.
       unfold gv2gvs. simpl. auto.
 Opaque gv2gvs. 
-Qed.
-
-Lemma free_allocas_preserves_wf_Mem: forall maxb td als Mem Mem',
-  wf_Mem maxb td Mem -> free_allocas td Mem als = ret Mem' -> 
-  wf_Mem maxb td Mem'.
-Proof.
-  induction als; simpl; intros.
-    inv H0. auto.
-
-    inv_mbind.
-    symmetry in HeqR.
-    eapply free_preserves_wf_Mem in HeqR; eauto.
-Qed.
-
-Lemma free_allocas_preserves_wf_als : forall maxb TD als als0 M M'
-  (Hfree: free_allocas TD M als0 = ret M') 
-  (Hwf: wf_als maxb M als),
-  wf_als maxb M' als.
-Proof.
-  induction als0; simpl; intros.
-    inv Hfree. auto.
-
-    inv_mbind.
-    symmetry in HeqR.
-    eapply free_preserves_wf_als in HeqR; eauto.
 Qed.
 
 Lemma preservation_return : forall maxb pinfo (HwfPI : WF_PhiInfo pinfo)  
@@ -2425,23 +1212,6 @@ Transparent inscope_of_cmd.
       eapply updateAddAL__wf_ECStack_head_tail; eauto.
 Transparent inscope_of_cmd inscope_of_tmn.
 
-Qed.
-
-Lemma BOP_preserves_no_alias: forall TD lc gl bop0 sz0 v1 v2 gvs3 gvsa, 
-  BOP TD lc gl bop0 sz0 v1 v2 = ret gvs3 ->
-  no_alias gvs3 gvsa.
-Proof.
-  intros.
-  unfold BOP in H.
-  inv_mbind'. eapply mbop_preserves_no_alias in H0; eauto.
-Qed.
-
-Lemma BOP_preserves_no_embedded_ptrs: forall TD lc gl bop0 sz0 v1 v2 gvs3, 
-  BOP TD lc gl bop0 sz0 v1 v2 = ret gvs3 -> no_embedded_ptrs gvs3.
-Proof.
-  intros.
-  unfold BOP in H.
-  inv_mbind'. eapply mbop_preserves_no_embedded_ptrs in H0; eauto.
 Qed.
 
 Lemma BOP__wf_GVs_in_ECs : forall (v : value) (v0 : value) (id1 : id) (bop0 : bop)
@@ -2785,16 +1555,6 @@ Proof.
       eapply valid_ptrs__trans; eauto. omega.
 Qed.
 
-Lemma undef__valid_lift_ptrs: forall g td t1 blk
-  (Hc2g : ret g = gundef td t1), valid_ptrs blk ($ g # t1 $).
-Proof.
-  unfold gundef. intros.
-  inv_mbind'.
-Local Transparent gv2gvs.
-  unfold gv2gvs. simpl. auto.
-Opaque gv2gvs.
-Qed.
-
 Lemma initializeFrameValues_preserves_wf_lc: forall TD la (gvs:list (GVsT DGVs))
   M (Hwf: forall gv, In gv gvs -> valid_ptrs (Mem.nextblock M) gv) 
   lc (Hinit : Opsem.initLocals TD la gvs = ret lc), wf_lc M lc.
@@ -2922,108 +1682,6 @@ Axiom callExternalFun_preserves_wf_EC : forall maxb pinfo TD M M' rid
 Definition wf_use_in_tail (pinfo:PhiInfo) (v:value) :=
 used_in_value (PI_id pinfo) v = false.
 
-Lemma store_preserves_mload_aux_inv: forall b1 b2 v2 m2 Mem' Mem ofs2 
-  (Hst: Mem.store m2 Mem b2 ofs2 v2 = ret Mem') mc ofs1 gvs0,
-  mload_aux Mem' mc b1 ofs1 = ret gvs0 ->
-  exists gvs2 : GenericValue,
-     mload_aux Mem mc b1 ofs1 = ret gvs2 /\
-     (forall v m,
-      In (v, m) gvs0 -> (v2, m2) = (v, m) \/ v = Vundef \/ In (v, m) gvs2).
-Proof.
-  induction mc; simpl; intros.
-    inv H. eauto.
-
-    inv_mbind'. symmetry in HeqR0.
-    apply IHmc in HeqR0.
-    destruct HeqR0 as [gvs2 [J1 J2]].
-    rewrite J1.
-   
-Admitted.
-
-Lemma mstore_aux_preserves_mload_aux_inv: forall mc b1 ofs1 gvs0 b2 gvs1 Mem' Mem ofs2,
-  mload_aux Mem' mc b1 ofs1 = ret gvs0 ->
-  mstore_aux Mem gvs1 b2 ofs2 = ret Mem' ->
-  exists gvs2 : GenericValue,
-     mload_aux Mem mc b1 ofs1 = ret gvs2 /\
-     (forall v m,
-      In (v, m) gvs0 -> In (v, m) gvs1 \/ v = Vundef \/ In (v, m) gvs2).
-Proof.
-  induction gvs1 as [|[]]; simpl; intros.
-    inv H0. exists gvs0. split; auto.
-  
-    inv_mbind'.
-    apply IHgvs1 in H2; auto.
-    destruct H2 as [gvs2 [J1 J2]].
-    symmetry in HeqR.
-    eapply store_preserves_mload_aux_inv in HeqR; eauto.
-    destruct HeqR as [gvs3 [J3 J4]].
-    exists gvs3.
-    split; auto.
-    intros.
-    apply J2 in H0.
-    destruct H0 as [H0 | [H0 | H0]]; subst; auto.
-    apply J4 in H0. 
-    destruct H0 as [H0 | [H0 | H0]]; subst; auto.
-Qed.
-
-Lemma mstore_preserves_mload_inv: forall TD Mem' gptr ty al gvs0 Mem gvs1 t
-  mp2 (H1 : mload TD Mem' gptr ty al = ret gvs0) align
-  (H2 : mstore TD Mem mp2 t gvs1 align = Some Mem'),
-  exists gvs2, mload TD Mem gptr ty al = ret gvs2 /\
-     (forall v m,
-      In (v, m) gvs0 -> In (v, m) gvs1 \/ v = Vundef \/ In (v, m) gvs2).
-Proof.
-  intros.
-  apply store_inv in H2.
-  destruct H2 as [b [ofs [J5 J4]]].
-  apply mload_inv in H1.
-  destruct H1 as [b1 [ofs1 [m1 [mc [J1 [J2 J3]]]]]]; subst.
-  unfold mload. simpl. rewrite J2.
-  symmetry in J5. apply GV2ptr_inv in J5. 
-  destruct J5 as [b2 [ofs2 [m2 [J6 J7]]]]; subst. inv J7.
-  eapply mstore_aux_preserves_mload_aux_inv; eauto.
-Qed.
-
-(*
-Lemma mstore_preserves_mload_inv: forall TD Mem' gptr ty al gvs0 Mem gv1 t
-  mp2 (H1 : mload TD Mem' gptr ty al = ret gvs0) align
-  (H2 : mstore TD Mem mp2 t gv1 align = Some Mem'),
-  Some gvs0 = gundef TD ty \/
-  gvs0 = gv1 \/
-  mload TD Mem gptr ty al = ret gvs0.
-Proof.
-  intros.
-  apply store_inv in H2.
-  destruct H2 as [b [ofs [J5 J4]]].
-  admit. (* mem prop *)
-Qed.
-*)
-
-Lemma mstore_preserves_mload: forall TD Mem' gptr ty al gvs0 Mem gv1 t
-  mp2 (H1 : mload TD Mem gptr ty al = ret gvs0) align
-  (H2 : mstore TD Mem mp2 t gv1 align = Some Mem')
-  (Hna: no_alias mp2 gptr),
-  mload TD Mem' gptr ty al = ret gvs0.
-Proof.
-  admit. (* mem prop *)
-Qed.
-
-Lemma mstore_preserves_mload': forall TD Mem' gptr ty al gvs0 Mem gv1 t
-  mp2 (H1 : mload TD Mem gptr ty al = ret gvs0) align
-  (H2 : mstore TD Mem mp2 t gv1 align = Some Mem'),
-  exists gvs1, mload TD Mem' gptr ty al = ret gvs1.
-Proof.
-  admit. (* mem prop *)
-Qed.
-
-Lemma no_alias_overlap: forall gvs1 gvs2 gvs0 gvsa,
-  no_alias gvs1 gvsa ->
-  no_alias gvs2 gvsa ->
-  (forall (v : val) (m : AST.memory_chunk),
-     In (v, m) gvs0 -> In (v, m) gvs1 \/ v = Vundef \/ In (v, m) gvs2) ->
-  no_alias gvs0 gvsa.
-Admitted.
-
 Lemma mstore_preserves_wf_defs_at_head : forall maxb pinfo TD M  
   M' gl v als lc gvs1 gv1 t mp2 align mps2 vp
   (Hgetop': Opsem.getOperandValue TD vp lc gl = ret mps2)
@@ -3043,7 +1701,8 @@ Proof.
   destruct Hlkp' as [J1 J2].
   split; auto.
     destruct J1 as [[mb [J11 [J12 J13]]] [J4 [gv J3]]]; subst.
-    split. exists mb. repeat split; auto. omega. admit. (* MemProp *)
+    split. 
+      erewrite <- nextblock_mstore; eauto.
     split.
       intros. 
       eapply mstore_preserves_mload_inv in H; eauto.
@@ -3075,7 +1734,8 @@ Proof.
   split; auto.
     clear J2.
     destruct J1 as [[mb [J11 [J12 J13]]] [J4 [gv J3]]]; subst.
-    split. exists mb. repeat split; auto. omega. admit. (* MemProp *)
+    split.
+      erewrite <- nextblock_mstore; eauto.
     split.
       intros.
       eapply mstore_preserves_mload_inv in Hst; eauto.
@@ -3087,19 +1747,6 @@ Proof.
       exists gv. 
       eapply mstore_preserves_mload; eauto.
       eapply operand__no_alias_with__tail; eauto.
-Qed.
-
-Lemma mstore_preserves_wf_lc: forall TD M' M mp2 t gv1 align
-  (Hst: mstore TD M mp2 t gv1 align = Some M') lc
-  (Hwf: wf_lc M lc),
-  wf_lc M' lc.
-Proof.
-  unfold wf_lc.
-  intros.
-  apply Hwf in H.
-  apply store_inv in Hst.
-  destruct Hst as [blk' [ofs' [J1 J2]]].
-  admit. (* Mem Props *)
 Qed.
 
 Lemma mstore_preserves_wf_ECStack_head_tail: forall maxb pinfo ECs TD M 
@@ -3122,7 +1769,7 @@ Proof.
   apply_clear Hwf in H. simpl in H. eapply_clear H in H3.
   destruct H3 as [[mb [J11 J12]] [J2 J3]]; subst.
   split.
-    exists mb. split; auto. admit. (* MemProp *)
+    erewrite <- nextblock_mstore; eauto.
   split; auto.
     intros.
     eapply mstore_preserves_mload_inv in Hst; eauto.
@@ -3171,14 +1818,6 @@ Proof.
         apply wf_ECStack_head_tail_cons__intro; auto.
 Qed.
 
-Lemma valid_ptrs_overlap: forall gvs1 gvs2 gvs0 bd,
-  valid_ptrs bd gvs1 ->
-  valid_ptrs bd gvs2 ->
-  (forall (v : val) (m : AST.memory_chunk),
-     In (v, m) gvs0 -> In (v, m) gvs1 \/ v = Vundef \/ In (v, m) gvs2) ->
-  valid_ptrs bd gvs0.
-Admitted.
-
 Lemma mstore_preserves_wf_Mem : forall maxb TD M mp2 t gv1 align M' gvs1 gl
   (Hwfgl: wf_globals maxb gl) (lc:DGVMap) v1 (Hwflc: wf_lc M lc) 
   (H0 : Opsem.getOperandValue TD v1 lc gl = Some gvs1)
@@ -3189,7 +1828,7 @@ Lemma mstore_preserves_wf_Mem : forall maxb TD M mp2 t gv1 align M' gvs1 gl
 Proof.
   intros. destruct Hwf as [J1 J2].
   assert (Mem.nextblock M = Mem.nextblock M') as EQ.
-    admit. (* Mem Props *)
+    erewrite nextblock_mstore; eauto.
   rewrite EQ in *.
   split; eauto.
     intros.
@@ -3200,18 +1839,6 @@ Proof.
       eapply operand__lt_nextblock with (M:=M) in H0; eauto.
         rewrite EQ in H0; auto.
         rewrite EQ; auto.
-Qed.
-
-Lemma mstore_preserves_wf_als : forall TD M mp2 t gv1 align M' maxb als
-  (Hst: mstore TD M mp2 t gv1 align = Some M') 
-  (Hwf: wf_als maxb M als),
-  wf_als maxb M' als.
-Proof.
-  intros. destruct Hwf as [J1 J2].
-  split; auto.
-    intros. 
-    apply J2 in H; auto.
-    admit. (* Mem Props *)
 Qed.
 
 Lemma mstore_preserves_wf_ECStack_head_tail': forall maxb pinfo ECs TD M 
@@ -3229,7 +1856,8 @@ Proof.
     eapply operand__no_alias_with__tail with (M:=M); eauto; simpl; auto.
   eapply_clear Hwf in H. simpl in H. eapply_clear H in H3.
   destruct H3 as [[mb [J11 J12]] [J2 J3]]; subst.
-  split. exists mb. split; auto. admit. (* MemProp *)
+  split.
+    erewrite <- nextblock_mstore; eauto.
   split; auto.
     intros.
     eapply mstore_preserves_mload_inv in Hst; eauto.
@@ -3237,13 +1865,6 @@ Proof.
     apply J3 in H3.
     eapply no_alias_overlap with (gvs1:=gv1); eauto.
 Qed.
-
-Lemma malloc_preserves_mload_inv: forall TD M M' mb align0 gn tsz 
-  (Hal : malloc TD M tsz gn align0 = ret (M', mb))
-  gptr gvs1 ty al 
-  (H : mload TD M' gptr ty al = ret gvs1),
-  mload TD M gptr ty al = ret gvs1 \/ ret gvs1 = gundef TD ty.
-Admitted. (* MemProp *)
 
 Lemma malloc_preserves_wf_ECStack_head_tail : forall maxb pinfo ECs TD M tsz gn 
   align0 M' lc mb t id0
@@ -3258,19 +1879,26 @@ Proof.
   intros. apply Hwf in H. destruct ec0. intros.
   eapply_clear H in H1.
   destruct H1 as [[mb' [J11 J12]] [J2 J3]]; subst; eauto.
-  split. exists mb'. split; auto. admit. (* MemProp *)
+  assert (maxb < mb' < Mem.nextblock M') as W.
+    erewrite <- nextblock_malloc; eauto. omega.
+  split; eauto.
   split.
     intros.
     destruct (id_dec id0 id1); subst.
       rewrite lookupAL_updateAddAL_eq in H. inv H.
-      admit. (* MemProp mb'<M.next=mb *)
+      rewrite simpl_blk2GV. rewrite simpl_blk2GV.
+      simpl. apply malloc_result in Hmlc. subst.
+      split; auto.
+      split; auto.
+      clear - J12.
+      intro J. subst. omega.
 
       rewrite <- lookupAL_updateAddAL_neq in H; eauto.
 
     intros.
     eapply malloc_preserves_mload_inv in Hmlc; eauto.
     destruct Hmlc as [G | G]; subst; eauto.
-      eapply undef_disjoint_with_ptr; eauto.
+      eapply undefs_disjoint_with_ptr; eauto.
 Qed.
 
 Lemma malloc_preserves_wf_defs_in_tail : forall maxb pinfo TD M  
@@ -3287,14 +1915,16 @@ Proof.
   split; auto.
     clear J2.
     destruct J1 as [[mb' [J11 [J12 J13]]] [J4 [gv J3]]]; subst.
-    split. exists mb'. repeat split; auto. omega. admit. (* MemProp *)
+    assert (maxb < mb' < Mem.nextblock M') as W.
+      erewrite <- nextblock_malloc; eauto. omega.
+    split; eauto.
     split.
       intros.
       eapply malloc_preserves_mload_inv in H0; eauto.
       destruct H0 as [G | G]; subst; eauto.
-        eapply undef_disjoint_with_ptr; eauto.
+        eapply undefs_disjoint_with_ptr; eauto.
 
-      exists gv. admit. (* Mem Prop *)
+      exists gv. eapply malloc_preserves_mload; eauto.
 Qed.
 
 Lemma malloc_preserves_wf_lc_in_tail: forall TD M M' tsz gn align0 mb lc
@@ -3302,8 +1932,10 @@ Lemma malloc_preserves_wf_lc_in_tail: forall TD M M' tsz gn align0 mb lc
   (Hwf: wf_lc M lc), wf_lc M' lc.
 Proof.
   unfold wf_lc.
-  intros.
-  admit. (* Mem Props *)
+  intros. apply Hwf in H.
+  eapply valid_ptrs__trans; eauto.
+  erewrite <- nextblock_malloc with (M':=M'); eauto. 
+  omega.
 Qed.
 
 Lemma malloc_preserves_wf_ECStack_head_tail' : forall maxb pinfo ECs TD M tsz gn 
@@ -3317,12 +1949,14 @@ Proof.
   intros. apply Hwf in H. destruct ec0. intros.
   eapply_clear H in H1.
   destruct H1 as [[mb' [J11 J12]] [J2 J3]]; subst; eauto.
-  split. exists mb'. split; auto. admit. (* MemProp *)
+  assert (maxb < mb' < Mem.nextblock M') as W.
+    erewrite <- nextblock_malloc; eauto. omega.
+  split; eauto.
   split; eauto.
     intros.
     eapply malloc_preserves_mload_inv in Hmlc; eauto.
     destruct Hmlc as [G | G]; subst; eauto.
-      eapply undef_disjoint_with_ptr; eauto.
+      eapply undefs_disjoint_with_ptr; eauto.
 Qed.
 
 Lemma malloc_preserves_wf_ECStack_in_tail : forall maxb pinfo TD M tsz gn align0 
@@ -3341,45 +1975,6 @@ Proof.
     split; auto.
       destruct a. simpl in *.
       eapply malloc_preserves_wf_ECStack_head_tail'; eauto.
-Qed.
-
-Lemma malloc_preserves_wf_Mem : forall maxb TD M tsz gn align0 M' mb
-  (Hmlc: malloc TD M tsz gn align0 = ret (M', mb))
-  (Hwf: wf_Mem maxb TD M),
-  wf_Mem maxb TD M'.
-Proof.
-  intros. destruct Hwf as [J1 J2].
-  assert (Mem.nextblock M + 1 = Mem.nextblock M') as EQ.
-    admit. (* Mem Props *)
-  split.
-    rewrite <- EQ.
-    intros.
-    eapply malloc_preserves_mload_inv in H; eauto.
-    destruct H as [G | G]; subst; eauto.
-      apply J1 in G. eapply valid_ptrs__trans; eauto. omega.
-      eapply undef_valid_ptrs; eauto.
- 
-    omega.
-Qed.
-
-Lemma malloc_preserves_wf_als : forall maxb TD M M' tsz gn align0 mb als
-  (Hmalloc: malloc TD M tsz gn align0 = ret (M', mb)) 
-  (Hwf: wf_als maxb M als),
-  wf_als maxb M' (mb::als).
-Proof.
-  intros. destruct Hwf as [J1 J2].
-  split.
-    constructor; auto.
-      intro J. apply J2 in J.
-      admit. (* Mem Props *)
-
-    intros. 
-    simpl in H. 
-    destruct H as [H | H]; subst.
-      admit. (* Mem Props *)
-
-      apply J2 in H.
-      admit. (* Mem Props *)
 Qed.
 
 Lemma impure_cmd_updated_preserves_wf_EC : forall maxb pinfo TD M M' lc F B 
@@ -3460,7 +2055,7 @@ Proof.
         eapply wf_defs_eq; eauto.
 Qed.
 
-Lemma valid_ptrs__no_alias__fresh_ptr: forall bound TD mb t (Hbd: bound < mb) 
+Lemma valid_ptrs__no_alias__fresh_ptr: forall bound TD mb t (Hbd: bound <= mb) 
   gvs, valid_ptrs bound gvs -> 
   no_alias gvs ($ blk2GV TD mb # typ_pointer t $).
 Proof.
@@ -3475,31 +2070,31 @@ Proof.
       intro J. subst. contradict H; omega.
 Qed.
 
-Lemma ptr_no_alias__no_alias_with_blk : forall b i0 m gvs2,
-  no_alias [(Vptr b i0, m)] gvs2 -> no_alias_with_blk gvs2 b.
-Proof. 
-  induction gvs2 as [|[]]; simpl; intros; auto.
-    destruct v; auto.
-    destruct H. destruct H.
-    split; auto.
-Qed.
-
-Lemma no_alias_sym: forall gvs2 gvs1, no_alias gvs1 gvs2 -> no_alias gvs2 gvs1.
+Lemma mload_aux_alloc_same': forall M M' lo hi b 
+  (Hal : Mem.alloc M lo hi = (M', b)) mc ofs,
+  exists gvs1, mload_aux M' mc b ofs = ret gvs1 /\ 
+    forall v m, In (v, m) gvs1 -> v = Vundef.
 Proof.
-  induction gvs1 as [|[]]; simpl; intros; auto.
-    simpl_env in H.
-    apply no_alias_split in H.
-    destruct H as [H1 H2].
-    destruct v; auto.
+  induction mc; simpl; intros.
+    exists nil. 
     split; auto.
-      apply ptr_no_alias__no_alias_with_blk in H1; auto.
-Qed.
+      intros. inv H.
+Admitted.
+
+Lemma mload_aux_malloc_same': forall TD M M' mb align0 gn tsz mc
+  (Hal : malloc TD M tsz gn align0 = ret (M', mb)),
+  exists gvs1, mload_aux M' mc mb (Int.signed 31 (Int.repr 31 0)) = ret gvs1.
+Proof.
+  intros. 
+  apply malloc_inv in Hal.
+  destruct Hal as [n [J1 [J2 J3]]].
+Admitted.
 
 Lemma alloca_preserves_wf_defs_at_head : forall maxb pinfo TD M  
   M' gl als lc t v
   (Hwfgl: wf_globals maxb gl) mb id0 tmn align0 cs cs1' l1 ps1 F gn tsz
   (Hal: malloc TD M tsz gn align0 = ret (M', mb)) (HwfM: wf_Mem maxb TD M)
-  (Hwflc : wf_lc M lc),
+  (Hwflc : wf_lc M lc) (Hsize: getTypeAllocSize TD t = ret tsz),
   forall ids0,
    F = PI_f pinfo ->
    inscope_of_pc F
@@ -3518,21 +2113,33 @@ Proof.
     inv Hlkp.
     split.
       split.
-        exists mb. admit. (* WF, MemProp *)
+        exists mb. 
+        rewrite simpl_blk2GV. rewrite simpl_blk2GV. 
+        split; auto. simpl.
+        split; auto. 
+          erewrite <- nextblock_malloc; eauto.
+          apply malloc_result in Hal. subst. 
+          destruct HwfM. omega.
       split.
         intros.
         assert (mload TD M gptr ty al = ret gvs1 \/
-                Some gvs1 = gundef TD ty) as J.
+                forall v m, In (v, m) gvs1 -> v = Vundef) as J.
           eapply malloc_preserves_mload_inv; eauto.
         destruct J as [J | J].
           destruct HwfM as [HwfM _].
           apply HwfM in J.
           eapply valid_ptrs__no_alias__fresh_ptr; eauto.
-          admit. (* MemProp *)
+          apply malloc_result in Hal. subst. omega.
 
-          eapply undef_disjoint_with_ptr; eauto.
+          eapply undefs_disjoint_with_ptr; eauto.
 
-        admit. (* MemProp by Hal. *)
+        rewrite simpl_blk2GV. 
+        unfold mload. simpl.
+        assert (exists mc, flatten_typ TD (PI_typ pinfo) = Some mc) as J.
+          admit. (* wfPI *)
+        destruct J as [mc J].
+        rewrite J.
+        eapply mload_aux_malloc_same'; eauto.
 
       intros.
       unfold wf_non_alloca_GVs.
@@ -3540,7 +2147,7 @@ Proof.
       rewrite <- lookupAL_updateAddAL_neq in Hlk0; auto.
       apply Hwflc in Hlk0.
       eapply valid_ptrs__no_alias__fresh_ptr; eauto.
-      admit. (* MemProp *)
+      apply malloc_result in Hal. subst. omega.
 
     rewrite <- lookupAL_updateAddAL_neq in Hlkp; auto.
     simpl in Hpindom.
@@ -3551,17 +2158,21 @@ Proof.
     split.
       destruct J1 as [[mb' [J31 [J32 J33]]] [J4 [gv J5]]]; subst.
       split.
-        exists mb'. split; auto. simpl. split; auto. admit. (* MemProp *)
+        exists mb'. 
+        split; auto. simpl.
+        split; auto. 
+          erewrite <- nextblock_malloc; eauto.
+          omega.
       split.
         intros.
         assert (mload TD M gptr ty al = ret gvs1 \/
-                Some gvs1 = gundef TD ty) as J.
+                forall v m, In (v, m) gvs1 -> v = Vundef) as J.
           eapply malloc_preserves_mload_inv; eauto.
         destruct J as [J | J]; eauto.
-          eapply undef_disjoint_with_ptr; eauto.
+          eapply undefs_disjoint_with_ptr; eauto.
 
-        exists gv. admit. (* MemProp by Hal. *)
-
+        eapply malloc_preserves_mload in Hal; eauto.
+       
       intros.
       unfold wf_non_alloca_GVs.
       destruct (id_dec id1 (PI_id pinfo)); auto.
@@ -3571,7 +2182,7 @@ Proof.
         apply Hwflc in Hlkp'.
         apply no_alias_sym.
         eapply valid_ptrs__no_alias__fresh_ptr; eauto.
-        admit. (* MemProp *)
+        apply malloc_result in Hal. subst. omega.
 
         rewrite <- lookupAL_updateAddAL_neq in Hlk0; auto.
         apply J2 in Hlk0.
@@ -3583,12 +2194,12 @@ Lemma malloc_preserves_wf_defs_at_head : forall maxb pinfo TD M
   M' gl als lc t v
   (Hwfgl: wf_globals maxb gl) mb id0 tmn align0 cs cs1' l1 ps1 F gn tsz
   (Hal: malloc TD M tsz gn align0 = ret (M', mb)) (HwfM: wf_Mem maxb TD M)
-  (Hwflc : wf_lc M lc),
+  (Hwflc : wf_lc M lc) (Hneq: id0 <> PI_id pinfo),
   forall ids0,
    F = PI_f pinfo ->
    inscope_of_pc F
      (block_intro l1 ps1 (cs1' ++ insn_malloc id0 t v align0 :: cs) tmn)
-     (insn_alloca id0 t v align0 :: cs) tmn = ret ids0 ->
+     (insn_malloc id0 t v align0 :: cs) tmn = ret ids0 ->
    wf_defs maxb pinfo TD M lc ids0 als ->
    wf_defs maxb pinfo TD M'
      (updateAddAL (GVsT DGVs) lc id0
@@ -3597,54 +2208,27 @@ Lemma malloc_preserves_wf_defs_at_head : forall maxb pinfo TD M
 Proof.
   intros. unfold wf_defs. 
   intros gvsa Hpindom Hlkp.
-  destruct (id_dec id0 (PI_id pinfo)); subst.
-    rewrite lookupAL_updateAddAL_eq in Hlkp.
-    inv Hlkp.
-    split.
-      split.
-        exists mb. admit. (* WF, MemProp *)
-      split.
-        intros.
-        assert (mload TD M gptr ty al = ret gvs1 \/
-                Some gvs1 = gundef TD ty) as J.
-          eapply malloc_preserves_mload_inv; eauto.
-        destruct J as [J | J].
-          destruct HwfM as [HwfM _].
-          apply HwfM in J.
-          eapply valid_ptrs__no_alias__fresh_ptr; eauto.
-          admit. (* MemProp *)
-
-          eapply undef_disjoint_with_ptr; eauto.
-
-        admit. (* MemProp by Hal. *)
-
-      intros.
-      unfold wf_non_alloca_GVs.
-      destruct (id_dec id0 (PI_id pinfo)); auto.
-      rewrite <- lookupAL_updateAddAL_neq in Hlk0; auto.
-      apply Hwflc in Hlk0.
-      eapply valid_ptrs__no_alias__fresh_ptr; eauto.
-      admit. (* MemProp *)
-
-    rewrite <- lookupAL_updateAddAL_neq in Hlkp; auto.
-    simpl in Hpindom.
-    destruct Hpindom as [Hpindom | Hpindom]; subst; try congruence.
-    assert (Hlkp':=Hlkp).
-    apply H1 in Hlkp; auto.
-    destruct Hlkp as [J1 J2].
-    split.
+  rewrite <- lookupAL_updateAddAL_neq in Hlkp; auto.
+  simpl in Hpindom.
+  destruct Hpindom as [Hpindom | Hpindom]; subst; try congruence.
+  assert (Hlkp':=Hlkp).
+  apply H1 in Hlkp; auto.
+  destruct Hlkp as [J1 J2].
+  split.
       destruct J1 as [[mb' [J31 [J32 J33]]] [J4 [gv J5]]]; subst.
       split.
-        exists mb'. simpl. repeat split; auto. omega. admit. (* MemProp *)
+        erewrite <- nextblock_malloc; eauto.
+        exists mb'. split; auto. split; auto. omega. 
+
       split.
         intros.
         assert (mload TD M gptr ty al = ret gvs1 \/
-                Some gvs1 = gundef TD ty) as J.
+                forall v m, In (v, m) gvs1 -> v = Vundef) as J.
           eapply malloc_preserves_mload_inv; eauto.
         destruct J as [J | J]; eauto.
-          eapply undef_disjoint_with_ptr; eauto.
+          eapply undefs_disjoint_with_ptr; eauto.
 
-        exists gv. admit. (* MemProp by Hal. *)
+        eapply malloc_preserves_mload in Hal; eauto.
 
       intros.
       unfold wf_non_alloca_GVs.
@@ -3655,7 +2239,7 @@ Proof.
         apply Hwflc in Hlkp'.
         apply no_alias_sym.
         eapply valid_ptrs__no_alias__fresh_ptr; eauto.
-        admit. (* MemProp *)
+        apply malloc_result in Hal. subst. omega.
 
         rewrite <- lookupAL_updateAddAL_neq in Hlk0; auto.
         apply J2 in Hlk0.
@@ -3672,11 +2256,17 @@ Proof.
   intros.
   destruct (id_dec id0 id1); subst.
     rewrite lookupAL_updateAddAL_eq in H.
-    admit. (* Mem Props *)
+    inv H. rewrite simpl_blk2GV. simpl.
+    erewrite <- nextblock_malloc; eauto.
+    apply malloc_result in Hmalloc. subst.
+    split; auto.
+      omega.
 
     rewrite <- lookupAL_updateAddAL_neq in H; auto.
     apply Hwf in H.
-    admit. (* Mem Props *)
+    erewrite <- nextblock_malloc; eauto.
+    eapply valid_ptrs__trans; eauto.
+    omega.
 Qed.
 
 Ltac simpl_ctx Hinv HwfS1 :=
@@ -3721,11 +2311,13 @@ Case "sMalloc".
         intros. subst.
         apply wf_EC__wf_lc in HwfEC.
         eapply malloc_preserves_wf_defs_at_head with (tmn:=tmn); eauto.
+          admit. (* WF PI *)
         eapply malloc_preserves_wf_lc; eauto.
     split.
       eapply malloc_preserves_wf_ECStack_in_tail in H2; eauto.
       eapply malloc_preserves_wf_ECStack_head_tail in H2; eauto.
   split.
+    destruct HwfM1.
     eapply malloc_preserves_wf_als in H2; eauto.
       simpl_env in H2.
       apply wf_als_split in H2. destruct H2; auto.
@@ -3760,6 +2352,7 @@ Case "sAlloca".
       eapply malloc_preserves_wf_ECStack_in_tail in H2; eauto.
       eapply malloc_preserves_wf_ECStack_head_tail in H2; eauto.
   split.
+    destruct HwfM1.
     eapply malloc_preserves_wf_als in H2; eauto.
     eapply malloc_preserves_wf_Mem in H2; eauto.
 
